Typing.v
@@ -1,0 +1,125 @@
+(************************************************
+ *           Row Subtyping - Typing             *
+ *                 Leo White                    *
+ ************************************************)
+
+Set Implicit Arguments.
+Require Import LibLN Cofinite Definitions
+        Substitution Wellformedness Kinding.
+
+Hint Constructors typing.
+
+Lemma valid_scheme_empty : forall E T,
+    kinding E T knd_type ->
+    valid_scheme E (sch_empty T).
+Proof.
+  introv Hk.
+  apply valid_scheme_c with (L := \{}).
+  introv Hf.
+  fresh_length Hf as Hl.
+  destruct Xs; try discriminate; auto.
+Qed.
+
+Lemma typing_weakening : forall E F G t T,
+    typing (E & G) t T ->
+    valid_env (E & F & G) ->
+    typing (E & F & G) t T.
+Proof.
+  introv Ht Hv.
+  apply validated_typing in Ht.
+  remember (E & G) as EG.
+  generalize dependent E.
+  generalize dependent G.
+  generalize dependent F.
+  induction Ht; introv Heq Hv; subst;
+    eauto using valid_instance_weakening, binds_weakening,
+                kinding_weakening, subtype_weakening
+          with valid_env_regular.    
+  - apply typing_abs with (L := L \u dom E0 \u dom F \u dom G);
+      auto using kinding_weakening.
+    intros x Hn.
+    assert (valid_env (E0 & F & G & x ~: sch_empty T1))
+      as He by auto using valid_env_type_weakening.
+    rewrite <- concat_assoc.
+    rewrite <- concat_assoc in He.
+    auto using concat_assoc.
+  - apply typing_let
+      with (M := M) (L := L \u dom E0 \u dom F \u dom G).
+    + intros Xs Hl.
+      assert (valid_env (E0 & F & G & Xs ~::* M))
+        as He by auto using valid_env_kinds_weakening.
+      rewrite <- concat_assoc.
+      rewrite <- concat_assoc in He.
+      auto using concat_assoc.
+    + intros x Hl.
+      assert (valid_env (E0 & F & G & x ~: M))
+        as He by auto using valid_env_type_weakening.
+      rewrite <- concat_assoc.
+      rewrite <- concat_assoc in He.
+      auto using concat_assoc.
+  - apply typing_match
+      with (L := L \u dom E0 \u dom F \u dom G)
+           (T1 := T1) (T2 := T2) (T3 := T3) (T4 := T4)
+           (T5 := T5) (T6 := T6) (T7 := T7);
+      auto using kinding_weakening, subtype_weakening.
+    + intros x Hn.
+      assert
+        (valid_env (E0 & F & G & x ~: sch_empty (typ_variant T3)))
+        as He by auto using valid_env_type_weakening.
+      rewrite <- concat_assoc.
+      rewrite <- concat_assoc in He.
+      auto using concat_assoc.
+    + intros y Hn.
+      assert
+        (valid_env (E0 & F & G & y ~: sch_empty (typ_variant T5)))
+        as He by auto using valid_env_type_weakening.
+      rewrite <- concat_assoc.
+      rewrite <- concat_assoc in He.
+      auto using concat_assoc.
+  - apply typing_destruct
+      with (L := L \u dom E0 \u dom F \u dom G)
+           (T1 := T1) (T2 := T2) (T3 := T3);
+      auto using kinding_weakening, subtype_weakening.
+    intros x Hn.
+    assert
+      (valid_env (E0 & F & G & x ~: sch_empty T3))
+      as He by auto using valid_env_type_weakening.
+    rewrite <- concat_assoc.
+    rewrite <- concat_assoc in He.
+    auto using concat_assoc.
+Qed.
+
+Lemma typing_weakening_l : forall E F t T,
+    typing E t T ->
+    valid_env (E & F) ->
+    typing (E & F) t T.
+Proof.
+  introv Ht Hv.
+  rewrite <- concat_empty_r with (E := E & F).
+  apply typing_weakening; rewrite concat_empty_r; assumption.
+Qed.
+
+Lemma typing_typ_subst : forall E F X K S t T,
+    typing (E & X ~:: K & F) t T ->
+    kinding E S K ->
+    typing (E & env_subst X S F) t (typ_subst X S T).
+Proof.
+  introv Ht Hk.
+  remember (E & X ~:: K & F) as EXF.
+  generalize dependent E.
+  generalize dependent F.
+  induction Ht; introv Heq Hk; subst.
+  - assert (binds x (bind_typ M) (E0 & X ~:: K & F))
+      as Hb by assumption.
+    destruct (binds_middle_inv Hb) as [?|[[_[_?]]|[?[??]]]].
+    + apply typing_var
+        with (M := sch_subst X S M)
+             (Us := (List.map (typ_subst X S) Us));
+        eauto using valid_env_typ_subst, valid_instance_typ_subst.
+      admit.
+      admit.
+    + discriminate.
+    + apply typing_var
+        with (M := M)
+             (Us := (List.map (typ_subst X S) Us));
+        eauto using valid_env_typ_subst, valid_instance_typ_subst.
